Self code review and clean up ArchSem

ArchSem/NondeterministicMonad.lean
@@ -1,4 +1,4 @@
-/-
+/-!
 This file provies monad types to help with non-deterministic state transitions
 used in various concurrency models.
 This file is an analogous of archsem-rocq's `Common/Exec.v`.
@@ -6,33 +6,55 @@ This file is an analogous of archsem-rocq's `Common/Exec.v`.
 
 namespace ArchSem.NondeterministicMonad
 
-/- Non-deterministic Except type can have multiple ok states and multiple errors. -/
+/--
+Non-deterministic Except.
+Finite non-determinisim only.
+In a non-deterministic transition system consisting of nodes from `α`
+and error states from `ε`, `oks` and `errors` represents the set of
+current ok states and error states respectivly.
+
+A common usecase is to specialize with `NExcept (σ × ε) (σ × α)` where
+`σ` represents a model state, and `α` a return value.
+We have some helper functions for working on a `NExcept` of this form.
+
+The order of the lists does not matter (TODO: implement equality instances).
+-/
 structure NExcept (ε α : Type) where
   oks : List α
   errors : List ε
 
 namespace NExcept
 
+/-- Return true iff any error states are present. -/
 def hasError (e : NExcept ε α) : Bool :=
   match e.errors with
   | [] => false
   | _ => true
 
+/-- Take the union of two state sets. -/
 def merge (m1 m2 : NExcept ε α) : NExcept ε α :=
   { oks := m1.oks ++ m2.oks, errors := m1.errors ++ m2.errors }
+
+/-- Nondeterministically choose an element from a list. -/
 def choose (s : List α) : NExcept ε α :=
   { oks := s, errors := [] }
-def error (e : ε) : NExcept ε α := { oks := [], errors := [e] }
 
+/-- The non-deterministic empty state. -/
+def empty : NExcept ε α :=
+  { oks := [], errors := [] }
+
+/-- Non-deterministically choose a `Fin n`. -/
 def chooseFin (n : Nat) : NExcept ε (Fin n) := choose (List.finRange n)
 
-def map (f : α → β) (m : NExcept ε α) : NExcept ε β := { oks := List.map f m.oks, errors := m.errors }
-def pure (v : α) : NExcept ε α := { oks := [v], errors := [] }
+/-- Non-deterministic state containing only the error `e`. -/
+def error (e : ε) : NExcept ε α := { oks := [], errors := [e] }
+
+def map (f : α → β) (m : NExcept ε α) : NExcept ε β :=
+  { oks := List.map f m.oks, errors := m.errors }
+def pure (v : α) : NExcept ε α :=
+  { oks := [v], errors := [] }
 def bind (m : NExcept ε α) (f : α → NExcept ε β) :=
   (m.oks.map f).foldr NExcept.merge { oks := [], errors := m.errors }
-
-def toExceptList (m : NExcept ε α) : List (Except ε α) :=
-  (m.oks.map Except.ok) ++ (m.errors.map Except.error)
 
 instance : Functor (NExcept ε) where
   map := map
@@ -41,21 +63,23 @@ instance : Monad (NExcept ε) where
   pure := pure
   bind := bind
 
+/-- Lift a deterministic state into a non-deterministic. -/
 instance : MonadLift (Except ε) (NExcept ε) where
   monadLift r := match r with
     | .ok a => { oks := [a], errors := [] }
     | .error e => { oks := [], errors := [e] }
 
+/-- Return all states in a list. Arbitrary order. -/
+def toExceptList (m : NExcept ε α) : List (Except ε α) :=
+  (m.oks.map Except.ok) ++ (m.errors.map Except.error)
+
+/-- Return all states paired with values in a list. -/
 def toStatefulExceptList (m : NExcept (σ × ε) (σ × α)) : List (σ × Except ε α) :=
   List.append
     (m.oks.map (fun (s, r) => (s, Except.ok r)))
     (m.errors.map (fun (s, err) => (s, Except.error err)))
-def toStateExceptList (m : NExcept (σ × ε) (σ × α)) : List (Except σ σ) :=
-  List.append
-    (m.oks.map (fun (s, _r) => Except.ok s))
-    (m.errors.map (fun (s, _err) => Except.error s))
-def successStateList (m : NExcept (σ × ε) (σ × α)) : List σ :=
-  m.oks.map (fun (s, _r) => s)
+
+/-- Map only the state of a `NExcept (σ × ε) (σ × α)`. -/
 def mapState (f : σ → σ') (r : NExcept (σ × ε) (σ × α)) : NExcept (σ' × ε) (σ' × α) :=
   { oks := r.oks.map (fun (s, a) => (f s, a))
   , errors := r.errors.map (fun (s, e) => (f s, e)) }
@@ -63,58 +87,80 @@ def mapState (f : σ → σ') (r : NExcept (σ × ε) (σ × α)) : NExcept (σ'
 end NExcept
 
 
-/- Non-deterministic Error State Monad (`Exec` in archsem-rocq). Finite non-determinisim only. -/
+/--
+Non-deterministic error state monad (`Exec` in archsem-rocq).
+i.e. a non-deterministic version of `EStateM`.
+Finite non-determinisim only.
+-/
 def NEStateM (ε σ α : Type) : Type := σ → NExcept (σ × ε) (σ × α)
 
 namespace NEStateM
 
+/-- Non-deterministically choose an element from the list, ignoring state. -/
 def choose (res : List α) : NEStateM σ ε α :=
   fun s => NExcept.choose (res.map (fun r => (s, r)))
+
+/-- Non-deterministically choose a `Fin n`, ignoring state. -/
+def chooseFin (n : Nat) : NEStateM σ ε (Fin n) :=
+  choose (List.finRange n)
+
+/-- Non-determistically throw all errors in the list, ignoring state. -/
 def throwErrors (errors : List ε) : NEStateM ε σ α :=
   fun s => { oks := [], errors := errors.map (fun e => (s, e))}
-def discard : NEStateM ε σ α :=
-  fun _ => { oks := [], errors := [] }
+
+/-- Non-deterministically throw a single error, ignoring state. -/
+def error (err : ε) : NEStateM ε σ α := throwErrors [err]
+
+def mapError (f : ε → ε') (m : NEStateM ε σ α) : NEStateM ε' σ α :=
+  fun s =>
+    let res := m s
+    { oks := res.oks
+    , errors := res.errors.map (fun (s', a) => (s', f a)) }
+
+def map (f : α → β) (m : NEStateM ε σ α) : NEStateM ε σ β :=
+  fun s => NExcept.map (fun (s, a) => (s, f a)) (m s)
+def pure (a : α) : NEStateM ε σ α :=
+  fun s => NExcept.pure (s, a)
 def bind (m : NEStateM ε σ α) (f : α → NEStateM ε σ β) : NEStateM ε σ β
   := fun s => do
     let (s', a) ← m s
     f a s'
-  
 
 instance : Functor (NEStateM σ ε) where
-  map f e := fun s =>  Functor.map (fun (s, a) => (s, f a)) (e s)
+  map := map
 
 instance : Monad (NEStateM ε σ) where
-  pure a := fun s => pure (s, a)
-  bind := NEStateM.bind
+  pure := pure
+  bind := bind
 
 instance : MonadState σ (NEStateM ε σ) where
-  get s := pure (s, s)
-  set s _ := pure (s, ())
+  get s := .pure (s, s)
+  set s _ := .pure (s, ())
   modifyGet f s :=
     let (a, s') := f s
-    pure (s', a)
+    .pure (s', a)
 
 instance : MonadLift (NExcept ε) (NEStateM ε σ) where
   monadLift r := fun s =>
     { oks := r.oks.map (fun a => (s, a))
     , errors := r.errors.map (fun e => (s, e)) }
 
-def error (err : ε) : NEStateM ε σ α := throwErrors [err]
-def chooseFin (n : Nat) : NEStateM σ ε (Fin n) := choose (List.finRange n)
-
-def discardNone : Option α → NEStateM σ ε α
-  | some a => pure a
-  | none => discard
-
+/-- Lift the monad into another state space using arbitrary getter and setter. -/
 def liftStateFull (getter : σ → σ') (setter : σ' → σ → σ)
     (inner : NEStateM ε σ' α) : NEStateM ε σ α :=
   fun s => NExcept.mapState (fun s' => setter s' s) (inner (getter s))
 
-def mapError (f : ε → ε') (m : NEStateM ε σ α) : NEStateM ε' σ α :=
-  fun s =>
-    let res := m s
-    { oks := res.oks
-    , errors := res.errors.map (fun (s', e) => (s', f e)) }
+/-- Transition to the non-deterministic empty state. -/
+def discard : NEStateM ε σ α :=
+  fun _ => NExcept.empty
+
+/--
+Return a pure value, ignoring state, if the option is some.
+discard all non-deterministic states if the option is none.
+-/
+def discardNone : Option α → NEStateM σ ε α
+  | some a => pure a
+  | none => discard
 
 end NEStateM
 
