ArchSem/Basic.lean
@@ -1,3 +1,13 @@
-import Out.Defs
+import ArchSem.Defs
+import ArchSem.NondeterministicMonad
+import ArchSem.TerminatingModel
+import ArchSem.LitmusTest.Basic
 
-def hello := "world"
+namespace ArchSem
+
+/-!
+At the moment this file is empty and the intended way to pull in
+dependencies is to import the other files on a need-by basis.
+-/
+
+end ArchSem
