ArchSem/LitmusTest/Defs.lean
@@ -1,55 +1,68 @@
-import ArchSem.TerminatingModel
 import Sail.ArchSem
+import ArchSem.TerminatingModel
 
-open ArchSem.TerminatingModel
 open Sail.ArchSem
+open ArchSem.TerminatingModel
 
 namespace ArchSem.LitmusTest
 
+variable [Arch] [ArchExtra]
+
+/-- All defined memory in a litmus test is labeled with a memory kind. -/
 inductive MemoryKind where
   | code
   | data
   | pageTable
 deriving Repr
 
+/-- Parse memory kinds from the '.archsem.toml' test format. -/
 def MemoryKind.fromString? : String → Option MemoryKind
   | "code" => some .code
   | "data" => some .data
   | "pagetable" => some .pageTable
   | _ => .none
 
-/-
- - We need to record `step` so we know what size to use when comparing with this
- - symbol in a final memory condition.
- -/
+/--
+Represents a contiguious defined block of memory with single MemoryKind
+and optionally labeled with symbol `sym`.
+-/
 structure MemoryBlock where
   addr : Nat
+  /-
+  We need to record `step` so we know what size to use when comparing with this
+  symbol in a final memory condition.
+  -/
   step : Nat
   data : List (BitVec 8)
   sym : Option String
   kind : MemoryKind
 deriving Repr
 
+/-- Write `MemoryBlock` onto `MemoryMap`. -/
 def MemoryBlock.insertIntoMemoryMap (mem : MemoryMap) (block : MemoryBlock)
     : MemoryMap :=
   block.data.foldl (fun (m, a) byte => (m.writeByte a byte, a + 1) ) (mem, block.addr)
   |> Prod.fst
 
+/-- A condition on an architecture-generic register checked at termination state. -/
 inductive FinalRegisterCondition where
   | regEq : RegValGen → FinalRegisterCondition
   | regNe : RegValGen → FinalRegisterCondition
 deriving Repr
 
+/-- A condition on an architecture-generic thread checked at termination state. -/
 structure FinalThreadCondition where
   tid : Tid
   regConditions : List (String × FinalRegisterCondition)
 deriving Repr
 
+/-- A condition on a memory location checked at termination state. -/
 inductive FinalMemoryWordCondition
-  | memEq : Nat → FinalMemoryWordCondition
-  | memNe : Nat → FinalMemoryWordCondition
+  | memEq (v : Nat)
+  | memNe (v : Nat)
 deriving Repr
 
+/-- A condition on memory to be checked at termination state. -/
 structure FinalMemoryCondition where
   sym : String
   addr : Nat
@@ -58,20 +71,26 @@ structure FinalMemoryCondition where
 deriving Repr
 
 /--
- - A condition the system should be in when it terminates.
- - In the toml format this is an element of [[outcome]].
- -/
+A condition to be checked on terminatin state.
+In the '.archsem.toml' format this is an element of [[outcome]].
+-/
 inductive FinalCondition where
   | observable : List FinalThreadCondition → List FinalMemoryCondition → FinalCondition
   | unobservable : List FinalThreadCondition → List FinalMemoryCondition → FinalCondition
 deriving Repr
 
+/-- A parsed '.archsem.toml' litmus test. -/
 structure TestRepr where
   arch : String
+  /-- Name of the test e.g. "MP". -/
   name : String
+  /-- List of initial register values for each thread. -/
   registers : List (List (String × RegValGen))
+  /-- List of blocks in initial memory. -/
   memory : List MemoryBlock
+  /-- List of register values for each thread to terminate at. -/
   termCond : List (List (String × RegValGen))
+  /-- List of conditions to check at the final state. -/
   finalConditions : List FinalCondition
 deriving Repr
 
@@ -79,7 +98,7 @@ deriving Repr
 Running a litmus test will result in this structure assuming no errors are
 encountered. It is strinctly a function of the final architecture states.
 -/
-inductive LitmusTestResult [ArchExtra]
+inductive LitmusTestResult
   | allowed
   | forbidden (reason : String)
 
